src/IMP2/IMP2_Expr.thy
@@ -24,32 +24,59 @@ fun bval :: "bexp => store => bool" where
   | "bval (Less a b)  s  = (aval a s < aval b s)"
   | "bval (Eq   a b)  s  = (aval a s = aval b s)"
 
+subsection \<open>Syntactic variable occurrence, parameterised over the predicate\<close>
+
+text \<open>
+  Both "does this expression mention a global?" and "does this expression
+  mention variable x?" are the same syntax-directed walk, differing only in
+  the leaf predicate on the mentioned name. Defining the walk once as
+  @{text "_where P"} and instantiating @{text P} to @{const is_global} (below)
+  or to an equality test (\<open>IMP2_Proc.aexp_mentions\<close>) avoids two copies of the
+  same recursion.
+\<close>
+
+fun aexp_n_mentions_where :: "(vname \<Rightarrow> bool) \<Rightarrow> AExp.aexp \<Rightarrow> bool" where
+  "aexp_n_mentions_where P (aexp.N _) = False"
+| "aexp_n_mentions_where P (aexp.V x) = P x"
+| "aexp_n_mentions_where P (AExp.aexp.Plus a b) = (aexp_n_mentions_where P a \<or> aexp_n_mentions_where P b)"
+
+fun aexp_mentions_where :: "(vname \<Rightarrow> bool) \<Rightarrow> aexp \<Rightarrow> bool" where
+  "aexp_mentions_where P (BaseN a) = aexp_n_mentions_where P a"
+| "aexp_mentions_where P (Plus a b) = (aexp_mentions_where P a \<or> aexp_mentions_where P b)"
+| "aexp_mentions_where P (Minus a b) = (aexp_mentions_where P a \<or> aexp_mentions_where P b)"
+| "aexp_mentions_where P (Times a b) = (aexp_mentions_where P a \<or> aexp_mentions_where P b)"
+
+fun bexp_n_mentions_where :: "(vname \<Rightarrow> bool) \<Rightarrow> BExp.bexp \<Rightarrow> bool" where
+  "bexp_n_mentions_where P (bexp.Bc _) = False"
+| "bexp_n_mentions_where P (BExp.bexp.Not b) = bexp_n_mentions_where P b"
+| "bexp_n_mentions_where P (BExp.bexp.And b1 b2) = (bexp_n_mentions_where P b1 \<or> bexp_n_mentions_where P b2)"
+| "bexp_n_mentions_where P (BExp.bexp.Less a b) = (aexp_n_mentions_where P a \<or> aexp_n_mentions_where P b)"
+
+fun bexp_mentions_where :: "(vname \<Rightarrow> bool) \<Rightarrow> bexp \<Rightarrow> bool" where
+  "bexp_mentions_where P (BaseB b) = bexp_n_mentions_where P b"
+| "bexp_mentions_where P (Not b) = bexp_mentions_where P b"
+| "bexp_mentions_where P (And b1 b2) = (bexp_mentions_where P b1 \<or> bexp_mentions_where P b2)"
+| "bexp_mentions_where P (Or b1 b2) = (bexp_mentions_where P b1 \<or> bexp_mentions_where P b2)"
+| "bexp_mentions_where P (Less a b) = (aexp_mentions_where P a \<or> aexp_mentions_where P b)"
+| "bexp_mentions_where P (Eq a b) = (aexp_mentions_where P a \<or> aexp_mentions_where P b)"
+
 subsection \<open>Syntactic global-variable occurrence\<close>
 
-fun aexp_n_mentions_global :: "AExp.aexp \<Rightarrow> bool" where
-  "aexp_n_mentions_global (aexp.N _) = False"
-| "aexp_n_mentions_global (aexp.V x) = is_global x"
-| "aexp_n_mentions_global (AExp.aexp.Plus a b) = (aexp_n_mentions_global a \<or> aexp_n_mentions_global b)"
+definition aexp_n_mentions_global :: "AExp.aexp \<Rightarrow> bool" where
+  "aexp_n_mentions_global = aexp_n_mentions_where is_global"
 
-fun aexp_mentions_global :: "aexp \<Rightarrow> bool" where
-  "aexp_mentions_global (BaseN a) = aexp_n_mentions_global a"
-| "aexp_mentions_global (Plus a b) = (aexp_mentions_global a \<or> aexp_mentions_global b)"
-| "aexp_mentions_global (Minus a b) = (aexp_mentions_global a \<or> aexp_mentions_global b)"
-| "aexp_mentions_global (Times a b) = (aexp_mentions_global a \<or> aexp_mentions_global b)"
+definition aexp_mentions_global :: "aexp \<Rightarrow> bool" where
+  "aexp_mentions_global = aexp_mentions_where is_global"
 
-fun bexp_n_mentions_global :: "BExp.bexp \<Rightarrow> bool" where
-  "bexp_n_mentions_global (bexp.Bc _) = False"
-| "bexp_n_mentions_global (BExp.bexp.Not b) = bexp_n_mentions_global b"
-| "bexp_n_mentions_global (BExp.bexp.And b1 b2) = (bexp_n_mentions_global b1 \<or> bexp_n_mentions_global b2)"
-| "bexp_n_mentions_global (BExp.bexp.Less a b) = (aexp_n_mentions_global a \<or> aexp_n_mentions_global b)"
+definition bexp_n_mentions_global :: "BExp.bexp \<Rightarrow> bool" where
+  "bexp_n_mentions_global = bexp_n_mentions_where is_global"
 
-fun bexp_mentions_global :: "bexp \<Rightarrow> bool" where
-  "bexp_mentions_global (BaseB b) = bexp_n_mentions_global b"
-| "bexp_mentions_global (Not b) = bexp_mentions_global b"
-| "bexp_mentions_global (And b1 b2) = (bexp_mentions_global b1 \<or> bexp_mentions_global b2)"
-| "bexp_mentions_global (Or b1 b2) = (bexp_mentions_global b1 \<or> bexp_mentions_global b2)"
-| "bexp_mentions_global (Less a b) = (aexp_mentions_global a \<or> aexp_mentions_global b)"
-| "bexp_mentions_global (Eq a b) = (aexp_mentions_global a \<or> aexp_mentions_global b)"
+definition bexp_mentions_global :: "bexp \<Rightarrow> bool" where
+  "bexp_mentions_global = bexp_mentions_where is_global"
+
+lemmas mentions_global_defs [simp] =
+  aexp_n_mentions_global_def aexp_mentions_global_def
+  bexp_n_mentions_global_def bexp_mentions_global_def
 
 text \<open>
   @{const aexp_mentions_global} / @{const bexp_mentions_global} classify whether an
@@ -78,19 +105,9 @@ lemma aval_eq_on_locals:
     and "\<And>x. \<not> is_global x \<Longrightarrow> s1 x = s2 x"
   shows "aval a s1 = aval a s2"
   using assms
-proof (induction a)
-  case (BaseN a)
-  then show ?case  using aexp_n_aval_eq_on_locals by fastforce
-next
-  case (Plus a b)
-  then show ?case by auto
-next
-  case (Minus a b)
-  then show ?case by auto
-next
-  case (Times a b)
-  then show ?case by auto
-qed
+  apply (induction a)
+  using aexp_n_aval_eq_on_locals
+  by fastforce+
 
 lemma bexp_n_bval_eq_on_locals:
   assumes ng: "\<not> bexp_n_mentions_global b"
@@ -108,9 +125,12 @@ next
   then show ?case by auto
 next
   case (Less a b)
-  then show ?case  apply(auto)
-    by (metis aexp_n_aval_eq_on_locals)+
-   
+  then have "AExp.aval a s1 = AExp.aval a s2"
+    and "AExp.aval b s1 = AExp.aval b s2"
+    using aexp_n_aval_eq_on_locals unfolding mentions_global_defs
+    by fastforce +
+  then show ?case
+    by simp
 qed
 
 lemma bval_eq_on_locals:
@@ -121,7 +141,7 @@ lemma bval_eq_on_locals:
 proof (induction b)
   case (BaseB a)
   then show ?case apply(auto)
-    using bexp_n_bval_eq_on_locals by blast +
+    using bexp_n_bval_eq_on_locals[unfolded mentions_global_defs] by blast +
 next
   case (Not b)
   then show ?case by auto
@@ -132,15 +152,20 @@ next
   case (Or b1 b2)
   then show ?case by auto
 next
-  case (Less a b')
-  then show ?case apply(auto)
-    by (metis aval_eq_on_locals)+
+  case (Less a b)
+  then have "aval a s1 = aval a s2" and "aval b s1 = aval b s2"
+    unfolding bexp_n_mentions_global_def apply(auto)
+    using aexp_mentions_global_def aval_eq_on_locals by presburger +
+  then show ?case
+    by auto
 next
-  case (Eq a b')
-  then show ?case apply(auto)
-    by (metis aval_eq_on_locals)+
+  case (Eq a b)
+  then have "aval a s1 = aval a s2" and "aval b s1 = aval b s2"
+    unfolding bexp_n_mentions_global_def apply(auto)
+    using aexp_mentions_global_def aval_eq_on_locals by presburger +
+  then show ?case 
+    by auto
 qed
-
 
 
 
